Veir/Dialects/LLVM/Byte/Examples.lean
@@ -1,0 +1,17 @@
+module
+
+import Std.Tactic.BVDecide
+public import Veir.Dialects.LLVM.Int.Basic
+import all Veir.Dialects.LLVM.Byte.Basic
+import all Veir.Dialects.LLVM.Byte.Lemmas
+
+namespace Veir.Dialects.LLVM.Byte
+
+example (w : Nat) (x y : Byte w) : x ||| y = y ||| x := by
+  simp only [or_eq]
+  simp [BitVec.or_comm (x.poison) (y.poison), BitVec.or_comm (x.val) (y.val)]
+
+example (x y : Byte 8) : x ||| y = y ||| x := by
+  bv_decide
+
+end Veir.Dialects.LLVM.Byte
